utp/utp_recursion.thy
@@ -119,15 +119,15 @@ lemma  wf_fixp_uinduct_pure_ueq_gen:
   assumes fixp_unfold: "fp B = B (fp B)"
   and              WF: "wf R"
   and     induct_step:
-          "\<And>f st. \<lbrakk>\<And>st'. (st',st) \<in> R  \<Longrightarrow> (((Pre \<and> \<lceil>e\<rceil>\<^sub>< =\<^sub>u \<guillemotleft>st'\<guillemotright>) \<Rightarrow> Post) \<sqsubseteq> f)\<rbrakk>
-               \<Longrightarrow> fp B = f \<Longrightarrow>((Pre \<and> \<lceil>e\<rceil>\<^sub>< =\<^sub>u \<guillemotleft>st\<guillemotright>) \<Rightarrow> Post) \<sqsubseteq> (B f)"
-        shows "((Pre \<Rightarrow> Post) \<sqsubseteq> fp B)"  
+          "\<And>f st. \<lbrakk>\<And>st'. (st',st) \<in> R  \<Longrightarrow> (((pre \<and> \<lceil>e\<rceil>\<^sub>< =\<^sub>u \<guillemotleft>st'\<guillemotright>) \<Rightarrow> post) \<sqsubseteq> f)\<rbrakk>
+               \<Longrightarrow> fp B = f \<Longrightarrow>((pre \<and> \<lceil>e\<rceil>\<^sub>< =\<^sub>u \<guillemotleft>st\<guillemotright>) \<Rightarrow> post) \<sqsubseteq> (B f)"
+        shows "((pre \<Rightarrow> post) \<sqsubseteq> fp B)"  
 proof -  
   { fix st
-    have "((Pre \<and> \<lceil>e\<rceil>\<^sub>< =\<^sub>u \<guillemotleft>st\<guillemotright>) \<Rightarrow> Post) \<sqsubseteq> (fp B)" 
+    have "((pre \<and> \<lceil>e\<rceil>\<^sub>< =\<^sub>u \<guillemotleft>st\<guillemotright>) \<Rightarrow> post) \<sqsubseteq> (fp B)" 
     using WF proof (induction rule: wf_induct_rule)
       case (less x)
-      hence "(Pre \<and> \<lceil>e\<rceil>\<^sub>< =\<^sub>u \<guillemotleft>x\<guillemotright> \<Rightarrow> Post) \<sqsubseteq> B (fp B)"
+      hence "(pre \<and> \<lceil>e\<rceil>\<^sub>< =\<^sub>u \<guillemotleft>x\<guillemotright> \<Rightarrow> post) \<sqsubseteq> B (fp B)"
         by (rule induct_step, rel_blast, simp)
       then show ?case
         using fixp_unfold by auto
@@ -141,7 +141,7 @@ text \<open> The next lemma shows that using substitution also work. However it 
         nor practical for proof automation ... \<close>
 
 lemma refine_usubst_to_ueq:
-  "vwb_lens E \<Longrightarrow> (Pre \<Rightarrow> Post)\<lbrakk>\<guillemotleft>st'\<guillemotright>/$E\<rbrakk> \<sqsubseteq> f\<lbrakk>\<guillemotleft>st'\<guillemotright>/$E\<rbrakk> = (((Pre \<and> $E =\<^sub>u \<guillemotleft>st'\<guillemotright>) \<Rightarrow> Post) \<sqsubseteq> f)"
+  "vwb_lens E \<Longrightarrow> (pre \<Rightarrow> post)\<lbrakk>\<guillemotleft>st'\<guillemotright>/$E\<rbrakk> \<sqsubseteq> f\<lbrakk>\<guillemotleft>st'\<guillemotright>/$E\<rbrakk> = (((pre \<and> $E =\<^sub>u \<guillemotleft>st'\<guillemotright>) \<Rightarrow> post) \<sqsubseteq> f)"
   by (rel_auto, metis vwb_lens_wb wb_lens.get_put)  
 
 text \<open> By instantiation of @{thm wf_fixp_uinduct_pure_ueq_gen} with @{term \<mu>} and lifting of the 
@@ -151,17 +151,17 @@ lemma mu_rec_total_pure_rule:
   assumes WF: "wf R"
   and     M: "mono B"  
   and     induct_step:
-          "\<And> f st.  \<lbrakk>(Pre \<and> (\<lceil>e\<rceil>\<^sub><,\<guillemotleft>st\<guillemotright>)\<^sub>u \<in>\<^sub>u \<guillemotleft>R\<guillemotright> \<Rightarrow> Post) \<sqsubseteq> f\<rbrakk>
-               \<Longrightarrow> \<mu> B = f \<Longrightarrow>(Pre \<and> \<lceil>e\<rceil>\<^sub>< =\<^sub>u \<guillemotleft>st\<guillemotright> \<Rightarrow> Post) \<sqsubseteq> (B f)"
-        shows "(Pre \<Rightarrow> Post) \<sqsubseteq> \<mu> B"  
-proof (rule wf_fixp_uinduct_pure_ueq_gen[where fp=\<mu> and Pre=Pre and B=B and R=R and e=e])
+          "\<And> f st.  \<lbrakk>(pre \<and> (\<lceil>e\<rceil>\<^sub><,\<guillemotleft>st\<guillemotright>)\<^sub>u \<in>\<^sub>u \<guillemotleft>R\<guillemotright> \<Rightarrow> post) \<sqsubseteq> f\<rbrakk>
+               \<Longrightarrow> \<mu> B = f \<Longrightarrow>(pre \<and> \<lceil>e\<rceil>\<^sub>< =\<^sub>u \<guillemotleft>st\<guillemotright> \<Rightarrow> post) \<sqsubseteq> (B f)"
+        shows "(pre \<Rightarrow> post) \<sqsubseteq> \<mu> B"  
+proof (rule wf_fixp_uinduct_pure_ueq_gen[where fp=\<mu> and pre=pre and B=B and R=R and e=e])
   show "\<mu> B = B (\<mu> B)"
     by (simp add: M def_gfp_unfold)
   show "wf R"
     by (fact WF)
-  show "\<And>f st. (\<And>st'. (st', st) \<in> R \<Longrightarrow> (Pre \<and> \<lceil>e\<rceil>\<^sub>< =\<^sub>u \<guillemotleft>st'\<guillemotright> \<Rightarrow> Post) \<sqsubseteq> f) \<Longrightarrow> 
+  show "\<And>f st. (\<And>st'. (st', st) \<in> R \<Longrightarrow> (pre \<and> \<lceil>e\<rceil>\<^sub>< =\<^sub>u \<guillemotleft>st'\<guillemotright> \<Rightarrow> post) \<sqsubseteq> f) \<Longrightarrow> 
                 \<mu> B = f \<Longrightarrow> 
-                (Pre \<and> \<lceil>e\<rceil>\<^sub>< =\<^sub>u \<guillemotleft>st\<guillemotright> \<Rightarrow> Post) \<sqsubseteq> B f"
+                (pre \<and> \<lceil>e\<rceil>\<^sub>< =\<^sub>u \<guillemotleft>st\<guillemotright> \<Rightarrow> post) \<sqsubseteq> B f"
     by (rule induct_step, rel_simp, simp)
 qed
 
@@ -169,31 +169,31 @@ lemma nu_rec_total_pure_rule:
   assumes WF: "wf R"
   and     M: "mono B"  
   and     induct_step:
-          "\<And> f st.  \<lbrakk>(Pre \<and> (\<lceil>e\<rceil>\<^sub><,\<guillemotleft>st\<guillemotright>)\<^sub>u \<in>\<^sub>u \<guillemotleft>R\<guillemotright> \<Rightarrow> Post) \<sqsubseteq> f\<rbrakk>
-               \<Longrightarrow> \<nu> B = f \<Longrightarrow>(Pre \<and> \<lceil>e\<rceil>\<^sub>< =\<^sub>u \<guillemotleft>st\<guillemotright> \<Rightarrow> Post) \<sqsubseteq> (B f)"
-        shows "(Pre \<Rightarrow> Post) \<sqsubseteq> \<nu> B"  
-proof (rule wf_fixp_uinduct_pure_ueq_gen[where fp=\<nu> and Pre=Pre and B=B and R=R and e=e])
+          "\<And> f st.  \<lbrakk>(pre \<and> (\<lceil>e\<rceil>\<^sub><,\<guillemotleft>st\<guillemotright>)\<^sub>u \<in>\<^sub>u \<guillemotleft>R\<guillemotright> \<Rightarrow> post) \<sqsubseteq> f\<rbrakk>
+               \<Longrightarrow> \<nu> B = f \<Longrightarrow>(pre \<and> \<lceil>e\<rceil>\<^sub>< =\<^sub>u \<guillemotleft>st\<guillemotright> \<Rightarrow> post) \<sqsubseteq> (B f)"
+        shows "(pre \<Rightarrow> post) \<sqsubseteq> \<nu> B"  
+proof (rule wf_fixp_uinduct_pure_ueq_gen[where fp=\<nu> and pre=pre and B=B and R=R and e=e])
   show "\<nu> B = B (\<nu> B)"
     by (simp add: M def_lfp_unfold)
   show "wf R"
     by (fact WF)
-  show "\<And>f st. (\<And>st'. (st', st) \<in> R \<Longrightarrow> (Pre \<and> \<lceil>e\<rceil>\<^sub>< =\<^sub>u \<guillemotleft>st'\<guillemotright> \<Rightarrow> Post) \<sqsubseteq> f) \<Longrightarrow> 
+  show "\<And>f st. (\<And>st'. (st', st) \<in> R \<Longrightarrow> (pre \<and> \<lceil>e\<rceil>\<^sub>< =\<^sub>u \<guillemotleft>st'\<guillemotright> \<Rightarrow> post) \<sqsubseteq> f) \<Longrightarrow> 
                 \<nu> B = f \<Longrightarrow> 
-                (Pre \<and> \<lceil>e\<rceil>\<^sub>< =\<^sub>u \<guillemotleft>st\<guillemotright> \<Rightarrow> Post) \<sqsubseteq> B f"
+                (pre \<and> \<lceil>e\<rceil>\<^sub>< =\<^sub>u \<guillemotleft>st\<guillemotright> \<Rightarrow> post) \<sqsubseteq> B f"
     by (rule induct_step, rel_simp, simp)
 qed
 
-text \<open>Since @{term "B ((Pre \<and> (\<lceil>E\<rceil>\<^sub><,\<guillemotleft>st\<guillemotright>)\<^sub>u\<in>\<^sub>u\<guillemotleft>R\<guillemotright> \<Rightarrow> Post)) \<sqsubseteq> B (\<mu> B)"} and 
+text \<open>Since @{term "B ((pre \<and> (\<lceil>E\<rceil>\<^sub><,\<guillemotleft>st\<guillemotright>)\<^sub>u\<in>\<^sub>u\<guillemotleft>R\<guillemotright> \<Rightarrow> post)) \<sqsubseteq> B (\<mu> B)"} and 
       @{term "mono B"}, thus,  @{thm mu_rec_total_pure_rule} can be expressed as follows\<close>
   
 lemma mu_rec_total_utp_rule: 
   assumes WF: "wf R"
     and     M: "mono B"  
     and     induct_step:
-    "\<And>st. (Pre \<and> \<lceil>e\<rceil>\<^sub>< =\<^sub>u \<guillemotleft>st\<guillemotright> \<Rightarrow> Post) \<sqsubseteq> (B ((Pre \<and> (\<lceil>e\<rceil>\<^sub><,\<guillemotleft>st\<guillemotright>)\<^sub>u \<in>\<^sub>u \<guillemotleft>R\<guillemotright> \<Rightarrow> Post)))"
-  shows "(Pre \<Rightarrow> Post) \<sqsubseteq> \<mu> B"  
+    "\<And>st. (pre \<and> \<lceil>e\<rceil>\<^sub>< =\<^sub>u \<guillemotleft>st\<guillemotright> \<Rightarrow> post) \<sqsubseteq> (B ((pre \<and> (\<lceil>e\<rceil>\<^sub><,\<guillemotleft>st\<guillemotright>)\<^sub>u \<in>\<^sub>u \<guillemotleft>R\<guillemotright> \<Rightarrow> post)))"
+  shows "(pre \<Rightarrow> post) \<sqsubseteq> \<mu> B"  
 proof (rule mu_rec_total_pure_rule[where R=R and e=e], simp_all add: assms)
-  show "\<And>f st. (Pre \<and> (\<lceil>e\<rceil>\<^sub><, \<guillemotleft>st\<guillemotright>)\<^sub>u \<in>\<^sub>u \<guillemotleft>R\<guillemotright> \<Rightarrow> Post) \<sqsubseteq> f \<Longrightarrow> \<mu> B = f \<Longrightarrow> (Pre \<and> \<lceil>e\<rceil>\<^sub>< =\<^sub>u \<guillemotleft>st\<guillemotright> \<Rightarrow> Post) \<sqsubseteq> B f"
+  show "\<And>f st. (pre \<and> (\<lceil>e\<rceil>\<^sub><, \<guillemotleft>st\<guillemotright>)\<^sub>u \<in>\<^sub>u \<guillemotleft>R\<guillemotright> \<Rightarrow> post) \<sqsubseteq> f \<Longrightarrow> \<mu> B = f \<Longrightarrow> (pre \<and> \<lceil>e\<rceil>\<^sub>< =\<^sub>u \<guillemotleft>st\<guillemotright> \<Rightarrow> post) \<sqsubseteq> B f"
     by (simp add: M induct_step monoD order_subst2)
 qed
 
@@ -201,10 +201,10 @@ lemma nu_rec_total_utp_rule:
   assumes WF: "wf R"
     and     M: "mono B"  
     and     induct_step:
-    "\<And>st. (Pre \<and> \<lceil>e\<rceil>\<^sub>< =\<^sub>u \<guillemotleft>st\<guillemotright> \<Rightarrow> Post) \<sqsubseteq> (B ((Pre \<and> (\<lceil>e\<rceil>\<^sub><,\<guillemotleft>st\<guillemotright>)\<^sub>u \<in>\<^sub>u \<guillemotleft>R\<guillemotright> \<Rightarrow> Post)))"
-  shows "(Pre \<Rightarrow> Post) \<sqsubseteq> \<nu> B"  
+    "\<And>st. (pre \<and> \<lceil>e\<rceil>\<^sub>< =\<^sub>u \<guillemotleft>st\<guillemotright> \<Rightarrow> post) \<sqsubseteq> (B ((pre \<and> (\<lceil>e\<rceil>\<^sub><,\<guillemotleft>st\<guillemotright>)\<^sub>u \<in>\<^sub>u \<guillemotleft>R\<guillemotright> \<Rightarrow> post)))"
+  shows "(pre \<Rightarrow> post) \<sqsubseteq> \<nu> B"  
 proof (rule nu_rec_total_pure_rule[where R=R and e=e], simp_all add: assms)
-  show "\<And>f st. (Pre \<and> (\<lceil>e\<rceil>\<^sub><, \<guillemotleft>st\<guillemotright>)\<^sub>u \<in>\<^sub>u \<guillemotleft>R\<guillemotright> \<Rightarrow> Post) \<sqsubseteq> f \<Longrightarrow> \<nu> B = f \<Longrightarrow> (Pre \<and> \<lceil>e\<rceil>\<^sub>< =\<^sub>u \<guillemotleft>st\<guillemotright> \<Rightarrow> Post) \<sqsubseteq> B f"
+  show "\<And>f st. (pre \<and> (\<lceil>e\<rceil>\<^sub><, \<guillemotleft>st\<guillemotright>)\<^sub>u \<in>\<^sub>u \<guillemotleft>R\<guillemotright> \<Rightarrow> post) \<sqsubseteq> f \<Longrightarrow> \<nu> B = f \<Longrightarrow> (pre \<and> \<lceil>e\<rceil>\<^sub>< =\<^sub>u \<guillemotleft>st\<guillemotright> \<Rightarrow> post) \<sqsubseteq> B f"
     by (simp add: M induct_step monoD order_subst2)
 qed
 
